

1. (a) Simplify: $9^{\log_3 n} = n^2$
 $\log_{10} 2^{n^3} = n^3 \cdot \log_{10} 2$ (Assume without proof) $n^3 - n^2 \log n \in \Theta(n^3)$
 $\log_{10} 2 \cdot n^3 \in \Theta(n^3)$

Polynomials: $\sqrt{n} < n^{1.5} < 9^{\log_3 n} < n^3 - n^2 \log n < (\log_{10} 2) \cdot n^3$

Compare $n!$, 4^{2n} , by Stirling's approximation $n! \sim \sqrt{2\pi n} \left(\frac{n}{e}\right)^n$ for big n

$$\lim_{n \rightarrow \infty} \frac{n!}{4^{2n}} = \lim_{n \rightarrow \infty} \sqrt{2\pi n} \left(\frac{n}{16e}\right)^n = \infty \Rightarrow \underline{n! \in \omega(4^{2n})} \Rightarrow \underline{4^{2n} < n!}$$

Compare $n!$, n^n

$$\lim_{n \rightarrow \infty} \frac{n!}{n^n} = \lim_{n \rightarrow \infty} \frac{\sqrt{2\pi n}}{e^n} = \lim_{n \rightarrow \infty} \frac{\frac{\sqrt{2\pi}}{2} \cdot \frac{1}{\sqrt{n}}}{e^n} = 0 \Rightarrow n! \in o(n^n) \Rightarrow \underline{n! < n^n}$$

Since polynomial < exponential in terms of order of growth

$$\log_{10} 2^{(n^3)} < 4^{2n}$$

So overall: $\sqrt{n} < n^{1.5} < 9^{\log_3 n} < n^3 - n^2 \log n < \log_{10} 2^{n^3} < 4^{2n} < n! < n^n$

(b) let $n = 3^x$ where $x \in \mathbb{Z}_+$

$$\begin{aligned} g(n) &= 3g\left(\frac{n}{3}\right) + n = G(x) = g(3^x) = 3g(3^{x-1}) + 3^x \\ &= 3G(x-1) + 3^x \\ &= 3(3G(x-2) + 3^{x-1}) + 3^x \\ &= 3^2 G(x-2) + 2 \cdot 3^x \\ &\vdots \\ &= 3^{x-1} \underbrace{G(1)}_{=g(3)=3} + (x-1)3^x \\ G(x) &= 3^x + (x-1)3^x \\ g(n) &= n + n \cdot (\log_3 n - 1) = \underline{n \log_3 n} \end{aligned}$$

2. Hypothesis: $\forall m \in \mathbb{Z}_{\geq 0}$, m can be expressed as a sum of finite set of Fib numbers, s.t. no two are the same and consecutive.
 Base Case: $m=0 = \text{Fib}(0)$ ✓
 $m=1 = \text{Fib}(1)$ ✓

Inductive step: Assume $\forall x < m$, the hypothesis is true.

$$\exists k \in \mathbb{Z}_+, \text{ s.t. } F_k \leq m < F_{k+1}, \quad F_{k+1} = F_k + F_{k-1}$$

$$\Leftrightarrow m < F_k + F_{k-1} \Leftrightarrow F_k + F_{k-1} \text{ cannot be summed to } m$$

let $m = F_k + m^*$, then $m^* < m$, by assumption

* m^* is sum of non-duplicate, non-consecutive Fib numbers.
 and m^* doesn't include F_{k-1} since $F_{k-1} + F_k > m$

therefore m is a sum of non-duplicate/non-consecutive Fib numbers.

By the principle of MI, the hypothesis is true.

3. let $f(n) = n$, $g(n) = n^2$, let $0 \leq \alpha, \beta < 1$ s.t. $\log n + \alpha = \lceil \log n \rceil$
 $n \in o(n^2)$ $\log n^2 + \beta = \lceil \log n^2 \rceil$

$$\lim_{n \rightarrow \infty} \frac{\lceil \log n \rceil}{\lceil \log n^2 \rceil} = \lim_{n \rightarrow \infty} \frac{\log n + \alpha}{\log n^2 + \beta} = \lim_{n \rightarrow \infty} \frac{\log n}{\log n^2} = \lim_{n \rightarrow \infty} \frac{\frac{1}{n}}{\frac{2}{n}} = \frac{1}{2} \neq 0$$

therefor $\lceil \log n \rceil \notin o(\lceil \log n^2 \rceil)$ (L'Hopital's Rule)

\Rightarrow not true